start 7.2

Chapter 7/Ex7_1.thy
@@ -2,6 +2,8 @@ theory Ex7_1 imports "~~/src/HOL/IMP/Big_Step" "~~/src/HOL/IMP/Small_Step" begin
 
 section "Chapter 7 exercises"
   
+subsection "7.1"
+  
 fun assigned :: "com \<Rightarrow> vname set" where
   "assigned (SKIP) = {}" |
   "assigned (Assign vname _) = {vname}" |
@@ -12,5 +14,39 @@ fun assigned :: "com \<Rightarrow> vname set" where
 lemma unassigned_is_unchanged:"\<lbrakk>(c,s) \<Rightarrow> t; x \<notin> assigned c\<rbrakk> \<Longrightarrow> s x = t x"
   apply(induction rule: big_step_induct)
   by auto
+
+subsection "7.2"
+
+fun skip :: "com \<Rightarrow> bool" where
+  "skip (SKIP) = True" |
+  "skip (Assign _ _) = False" |
+  "skip (Seq  c0 c1) = (skip c0 \<and> skip c1)" |
+  "skip (If   _ c0 c1) = (skip c0 \<and> skip c1)" |
+  "skip (While  _ com) = skip com"
+  
+lemma skip_like_SKIP: "skip c \<Longrightarrow> c \<sim> SKIP"
+proof(induction c)
+  case SKIP
+  then show ?case by simp
+next
+  case (Assign x1 x2)
+  then show ?case by simp
+next
+  case (Seq c1 c2)
+  then show ?case by fastforce
+next
+  case (If bexp c1 c2)
+  then show ?case
+    proof(cases "bval bexp s")
+      case True
+      then show ?thesis     try0 sorry
+    next
+      case False
+      then show ?thesis     try0 sorry
+    qed
+next
+  case (While x1 c)
+  then show ?case try0 sorry
+qed
   
 end
